test: LSP server verso tests
We add LSP tests for Verso documents; we reuse the core LSP testing
infrastructure from lean4 upstream. See `doc/dev/testing.md` there for
more details.

Co-authored-by: David Thrane Christiansen <david@lean-fro.org>

src/tests/TestMain.lean
@@ -153,6 +153,16 @@ def testBlog (_ : Config) : IO Unit := do
   if fails > 0 then
     throw <| .userError s!"{fails} blog tests failed"
 
+-- Interactive tests via the LSP server
+def testInteractive (_ : Config) : IO Unit := do
+  IO.println "Running interactive (LSP) tests..."
+  IO.println s!"current dir: {(← IO.Process.getCurrentDir)}"
+  -- We use the lower-level Process.spawn, which causes the subprocess to inherit the stdio
+  let child ← IO.Process.spawn { cmd := "src/tests/interactive/run_interactive.sh" }
+  let exitCode ← child.wait
+  if exitCode != 0 then
+    throw <| IO.userError s!"Interactive LSP tests failed with exit code {exitCode}"
+
 open Verso.Integration in
 def tests := [
   testSerialization,
@@ -165,7 +175,8 @@ def tests := [
     (extraFiles := [("src/tests/integration/extra-files-doc/test-data/shared", "shared")])
     (extraFilesTeX := [("src/tests/integration/extra-files-doc/test-data/TeX-only", "TeX-only")]),
   testTexOutput "front-matter-doc" FrontMatter.doc,
-  testZip
+  testZip,
+  testInteractive
 ]
 
 def getConfig (config : Config) : List String → IO Config
