src/tests/interactive/test-cases/inline_goals.lean
@@ -1,0 +1,24 @@
+import Verso
+import VersoManual
+
+theorem test0 : ∀ (n : Nat), n = n := by
+  intros
+     --^ textDocument/hover
+  rfl
+
+open Verso.Genre Manual InlineLean
+
+#doc (Manual) "Test for Goals in Inline Lean" =>
+
+We ship two tests for inline lean codeblocks:
+
+- show hover info over the constant in the codeblock
+- shows goals info on a proof
+
+```lean
+  --^ textDocument/hover
+theorem test : ∀ (n : Nat), n = n := by
+  intros
+     --^ $/lean/plainGoal
+  rfl
+```
